@prefix owl:  <http://www.w3.org/2002/07/owl#> .
@prefix rdf:  <http://www.w3.org/1999/02/22-rdf-syntax-ns#> .
@prefix rdfs: <http://www.w3.org/2000/01/rdf-schema#> .
@prefix xsd:  <http://www.w3.org/2001/XMLSchema#> .
@prefix sh:   <http://www.w3.org/ns/shacl#> .
# WARNING:
#
#    we will update the namespace associated with psh
#    with a dereferenceable uri before publishing the article
#
@prefix psh:  <http://www.example.org/ns/probabilistic-shacl#> .

################################################################################################

psh:
	a owl:Ontology ;
	rdfs:label "Probabilistic SHACL Validation"@en ;
	rdfs:comment "This vocabulary defines terms used to include and exploit probabilistic information in SHACL validation reports"@en .


psh:ValidationSummary 
    a rdfs:Class ;
    rdfs:label "Validation summary"@en ;
	rdfs:comment "The class of probabilistic validation summary"@en ;
	rdfs:subClassOf rdfs:Resource ;
	rdfs:isDefinedBy psh: .


psh:summary
    a rdf:Property ;
    rdfs:label "summary"@en ;
    rdfs:comment "The probabilistic validation results contained in a validation report."@en ;
    rdfs:domain sh:ValidationReport ;
    rdfs:range psh:ValidationSummary ;
    rdfs:isDefinedBy psh: .

psh:focusShape
    a rdf:Property ;
	rdfs:label "focus shape"@en ;
	rdfs:comment "The shape concerned by the results of the probabilistic validation"@en ;
	rdfs:domain sh:ValidationSummary ;
	rdfs:range sh:Shape ;
	rdfs:isDefinedBy psh: .

psh:numConfirmation
    a rdf:Property ;
    rdfs:label "number of confirmation"@en ;
    rdfs:comment "Specifies the number of nodes that confirm the current shape"@en ;
    rdfs:domain sh:ValidationSummary ;
    rdfs:range xsd:integer ;
    rdfs:isDefinedBy psh: .

psh:numViolation
    a rdf:Property ;
    rdfs:label "number of violation"@en ;
    rdfs:comment "Specifies the number of nodes that contradict the current shape"@en ;
    rdfs:domain sh:ValidationSummary ;
    rdfs:range xsd:integer ;
    rdfs:isDefinedBy psh: .

psh:referenceCardinality
    a rdf:Property ;
    rdfs:label "reference cardinality"@en ;
    rdfs:comment "Specifies the number of RDF triples tested during the validation of the current shape"@en ;
    rdfs:domain sh:ValidationSummary ;
    rdfs:range xsd:integer ;
    rdfs:isDefinedBy psh: .

psh:likelihood
    a rdf:Property ;
    rdfs:label "likelihood"@en ;
    rdfs:comment "Specifies the likelihood to observe the number of exceptions among the RDF triples tested (i.e. referenceCardinality)"@en ;
    rdfs:domain sh:ValidationSummary ;
    rdfs:range xsd:double ;
    rdfs:isDefinedBy psh: .

psh:generality
    a rdf:Property ;
    rdfs:label "likelihood"@en ;
    rdfs:comment "Specifies the representativeness of the current shape"@en ;
    rdfs:domain sh:ValidationSummary ;
    rdfs:range xsd:double ;
    rdfs:isDefinedBy psh: .
